

Theory of Machine Learning: Homework 3

1. We want to show that $A \subseteq B$ does not imply $N(A, \epsilon) \leq N(B, \epsilon)$.

Proof. We can provide a counterexample. Consider $A \subset \mathbb{R}$, $\epsilon > 0$. Let $A = \{0, \frac{3}{2}\epsilon\}$. The smallest ϵ -net that will cover A is itself, i.e. we need a ball of radius ϵ at both points in A to cover it, since they are farther than ϵ away from one another and cannot both be covered by a single ball. So $N(A, \epsilon) = 2$.

Create $B = A \cup \{\frac{3}{4}\epsilon\} = \{0, \frac{3}{4}\epsilon, \frac{3}{2}\epsilon\}$. Note that $|\frac{3}{4}\epsilon - 0| = \frac{3}{4}\epsilon$ and $|\frac{3}{4}\epsilon - \frac{3}{2}\epsilon| = \frac{3}{4}\epsilon$, so a single ball of radius ϵ placed at the new point, $\frac{3}{4}\epsilon$, will cover all of B . So smallest ϵ -net over B is $\{\frac{3}{4}\epsilon\} \implies N(B, \epsilon) = 1$.

So it is simultaneously true that $A \subseteq B$ and $N(A, \epsilon) > N(B, \epsilon)$.

QED

2. N/A

3. (a) We want to prove for any S and any $h, h' \in \mathcal{H}$ that $|E_S(h) - E_S(h')| \leq 4M \|h - h'\|_\infty$.

Proof.

$$\begin{aligned}
 |E_S(h) - E_S(h')| &= \left| [L_D(h) - \hat{L}_S(h)] - [L_D(h') - \hat{L}_S(h')] \right| \\
 &= \left| [L_D(h) - L_D(h')] + [\hat{L}_S(h') - \hat{L}_S(h)] \right| \\
 &\leq |[L_D(h) - L_D(h')]| + |\hat{L}_S(h') - \hat{L}_S(h)| \quad (\text{triangle inequality}) \\
 &= \left| \mathbb{E}_{z \sim D} [(h(x) - y)^2 - (h'(x) - y)^2] \right| + \left| \frac{1}{m} \sum_{i=1}^m [(h'(x_i) - y_i)^2 - (h(x_i) - y_i)^2] \right| \\
 &= \left| \mathbb{E}_{z \sim D} [h(x)^2 - 2h(x)y + y^2 - (h'(x)^2 - 2h'(x)y + y^2)] \right| + \left| \frac{1}{m} \sum_{i=1}^m [\dots] \right| \\
 &= \left| \mathbb{E}_{z \sim D} [(h(x)^2 - h'(x)^2) - 2y(h'(x) - h(x))] \right| + \left| \frac{1}{m} \sum_{i=1}^m [\dots] \right| \\
 &= \left| \mathbb{E}_{z \sim D} [(h(x) + h'(x))(h(x) - h'(x)) - 2y(h'(x) - h(x))] \right| + \left| \frac{1}{m} \sum_{i=1}^m [\dots] \right| \\
 &= \left| \mathbb{E}_{z \sim D} [(h(x) - h'(x))(h(x) + h'(x) - 2y)] \right| + \left| \frac{1}{m} \sum_{i=1}^m [\dots] \right| \\
 &\leq \left| \mathbb{E}_{z \sim D} \left[\max_{x \in \mathcal{X}} [h(x) - h'(x)] \cdot [(h(x) - y) + (h'(x) - y)] \right] \right| + \left| \frac{1}{m} \sum_{i=1}^m [\dots] \right| \quad (\text{monotonicity}) \\
 &\leq \left| \mathbb{E}_{z \sim D} [\|h - h'\|_\infty \cdot (M + M)] \right| + \left| \frac{1}{m} \sum_{i=1}^m [\dots] \right| \quad (\text{monotonicity}) \\
 &= 2M \|h - h'\|_\infty + \left| \frac{1}{m} \sum_{i=1}^m [\dots] \right| \\
 &\leq 2M \|h - h'\|_\infty + \left| \frac{1}{m} \sum_{i=1}^m 2M \|h - h'\|_\infty \right|, \quad \text{by the same process as above} \\
 &= 4M \|h - h'\|_\infty \\
 \implies |E_S(h) - E_S(h')| &\leq 4M \|h - h'\|_\infty
 \end{aligned}$$

QED

- (b) Assume $\mathcal{H} \subset \bigcup_{j=1}^k \mathcal{B}_j$. We want to show that

$$\Pr_{S \sim D^m} \left[\sup_{h \in \mathcal{H}} |E_S(h)| \geq \epsilon \right] \leq \sum_{j=1}^k \Pr_{S \sim D^m} \left[\sup_{h \in \mathcal{B}_j} |E_S(h)| \geq \epsilon \right]$$

Proof. Define $E = \{S : \sup_{h \in \mathcal{H}} |E_S(h)| \geq \epsilon\}$. Define $E_j = \{S : \sup_{h \in \mathcal{B}_j} |E_S(h)| \geq \epsilon\}$. Take any $S' \in E$. A sequence h_n must exist s.t. $\lim_{n \rightarrow \infty} |E_{S'}(h_n)| \rightarrow \sup_{h \in \mathcal{H}} |E_{S'}(h)|$. There are k sets covering \mathcal{H} . So, for at least one index j' , there should be a subsequence $h_{n_l} \in \mathcal{B}_{j'}$, i.e. there are infinitely many points occurring in one set $\mathcal{B}_{j'}$. So,

$$\sup_{h \in \mathcal{B}_{j'}} |E_{S'}(h)| \geq \lim_{l \rightarrow \infty} |E_{S'}(h_{n_l})| = \sup_{h \in \mathcal{H}} |E_{S'}(h)| \geq \epsilon$$

That is, for all $S \in E$, for some $j \in [k]$, $S \in E_j$. So, $E \subseteq \bigcup_{j=1}^k E_j$. So,

$$\begin{aligned} D^m \left(\{S : \sup_{h \in \mathcal{H}} |E_S(h)| \geq \epsilon\} \right) &\leq D^m \left(\bigcup_{j=1}^k \{S : \sup_{h \in \mathcal{B}_j} |E_S(h)| \geq \epsilon\} \right) \quad (\text{monotonicity of } D^m) \\ \implies D^m \left(\{S : \sup_{h \in \mathcal{H}} |E_S(h)| \geq \epsilon\} \right) &\leq \sum_{j=1}^k D^m \left(\{S : \sup_{h \in \mathcal{B}_j} |E_S(h)| \geq \epsilon\} \right) \quad (\text{union bound}) \end{aligned}$$

QED

- (c) Let \mathcal{B}_j be the intersection of \mathcal{H} with a ball of radius $\epsilon/(8M)$ w.r.t. the L^∞ norm, centered at h_j . We want to show that

$$\Pr \left[\sup_{h \in \mathcal{B}_j} |E_S(h)| \geq \epsilon \right] \leq \Pr [|E_S(h_j)| \geq \epsilon/2]$$

Proof. Define $E = \{S : \sup_{h \in \mathcal{B}_j} |E_S(h)| \geq \epsilon\}$. Define $E' = \{S : |E_S(h_j)| \geq \epsilon/2\}$. We know that $\forall h \in \mathcal{B}_j$, $\|h - h_j\|_\infty \leq \epsilon/(8M)$. Then

$$\begin{aligned} |E_S(h) - E_S(h_j)| &\leq 4M \|h - h_j\|_\infty \quad (\text{by part (a)}) \\ &\leq 4M \left(\frac{\epsilon}{8M} \right) \\ &= \epsilon/2 \end{aligned}$$

Since $||E_S(h)| - |E_S(h_j)|| \leq |E_S(h) - E_S(h_j)| \leq \epsilon/2$, we know that

$$\begin{aligned} |E_S(h)| - |E_S(h_j)| &\leq \epsilon/2 \\ \implies |E_S(h)| &\leq |E_S(h_j)| + \frac{\epsilon}{2} \end{aligned}$$

Now, pick any $S' \in E$. It is true that

$$\begin{aligned} \epsilon &\leq |E_{S'}(h)| \leq |E_{S'}(h_j)| + \frac{\epsilon}{2} \\ \implies \epsilon &\leq |E_{S'}(h_j)| + \frac{\epsilon}{2} \\ \implies \epsilon/2 &\leq |E_{S'}(h_j)| \end{aligned}$$

So, $E \subseteq E'$. Then, the monotonicity of D^m implies

$$D^m \left(\{S : \sup_{h \in \mathcal{B}_j} |E_S(h)| \geq \epsilon\} \right) \leq D^m (\{S : |E_S(h_j)| \geq \epsilon/2\})$$

QED

- (d) Let $k = N(\mathcal{H}, \|\cdot\|_\infty, \epsilon/(8M))$ be the covering number of \mathcal{H} by an ϵ -net $\{h_1, \dots, h_k\} \subset \mathcal{H}$. We will show a generalization bound using this net.

Proof. For every $i \in [m]$, define the r.v. $X_i = \frac{1}{m} (h_j(x_i) - y_i)^2$. Define $A_m = \sum_{i=1}^m X_i$.

Note that $|h_j(x) - y| \leq M \implies X_i \in \left[0, \frac{M^2}{m}\right]$. Then, by Hoeffding's inequality,

$$\begin{aligned} \Pr[A_m - \mathbb{E}[A_m] \geq \epsilon/2] &\leq \exp \left(\frac{-2(\epsilon/2)^2}{\sum_{i=1}^m (M^2/m - 0)^2} \right) \\ &= \exp \left(\frac{-2\epsilon^2}{4 \sum_{i=1}^m M^4/m^2} \right) \end{aligned}$$

$$\begin{aligned}
&= \exp\left(\frac{-\epsilon^2}{2M^4/m}\right) \\
&= \exp\left(\frac{-m\epsilon^2}{2M^4}\right)
\end{aligned}$$

It is therefore also true that

$$\Pr[A_m - \mathbb{E}[A_m] \leq -\epsilon/2] \leq \exp\left(\frac{-m\epsilon^2}{2M^4}\right)$$

Both events are disjoint, so we can take the union and sum the probabilities:

$$\Pr[|A_m - \mathbb{E}[A_m]| \geq \epsilon/2] \leq 2 \exp\left(\frac{-m\epsilon^2}{2M^4}\right)$$

Note that $A_m = \hat{L}_S(h_j)$ and $\mathbb{E}[A_m] = L_D(h_j)$. So,

$$|A_m - \mathbb{E}[A_m]| = |\mathbb{E}[A_m] - A_m| = |L_D(h_j) - \hat{L}_S(h_j)| = |E_S(h_j)|$$

Then, the prior inequality becomes:

$$\Pr[|E_S(h_j)| \geq \epsilon/2] \leq 2 \exp\left(\frac{-m\epsilon^2}{2M^4}\right)$$

We know from (b) and (c) that

$$\Pr\left[\sup_{h \in \mathcal{H}} |E_S(h)| \geq \epsilon\right] \leq \sum_{j=1}^k \Pr\left[\sup_{h \in \mathcal{B}_j} |E_S(h)| \geq \epsilon\right] \leq \sum_{j=1}^k \Pr[|E_S(h_j)| \geq \epsilon/2]$$

So, applying the result of Hoeffding's inequality, we get

$$\begin{aligned}
\Pr\left[\sup_{h \in \mathcal{H}} |E_S(h)| \geq \epsilon\right] &\leq \sum_{j=1}^k \Pr[|E_S(h_j)| \geq \epsilon/2] \\
&\leq \sum_{j=1}^k 2 \exp\left(\frac{-m\epsilon^2}{2M^4}\right) \\
&= k \cdot 2 \exp\left(\frac{-m\epsilon^2}{2M^4}\right) \\
\Rightarrow \Pr\left[\sup_{h \in \mathcal{H}} |E_S(h)| \geq \epsilon\right] &\leq N(\mathcal{H}, \|\cdot\|_\infty, \epsilon/(8M)) \cdot 2 \exp\left(\frac{-m\epsilon^2}{2M^4}\right)
\end{aligned}$$

QED